extracted/abort.ml
@@ -1,1 +1,0 @@
-let aBORT_FIXME _ = assert false
