theories/Translations/LustreToTiming.v
@@ -45,8 +45,8 @@ Definition translate_expr {ty} (e: Source.exp ty) (seed: ident): (
     Target.comb_exp ty (* init *)
     * Target.comb_exp ty (* step *)
     * ident (* New identifier origin *)
-    * (list binder) (* Variables created for pre *)
-    * (list Target.equation) (* pre equations *)
+    * list binder (* Variables created for pre *)
+    * list (binder * ident) (* pre equations *)
     (* Equations to merge with the regular equations *)
     (* for init: 
       prex = undef (a variable initialised later)
@@ -55,8 +55,8 @@ Definition translate_expr {ty} (e: Source.exp ty) (seed: ident): (
       prex = eqx (eqx being updated later with the current values)
     *)
     (* Equations NOT to be merged, but can be ordered separately *)
-    * (list Target.equation) (* init_post equations *)
-    * (list Target.equation) (* step_post equations *)
+    * list Target.equation (* init_post equations *)
+    * list Target.equation (* step_post equations *)
   ) :=
     Target.raw_to_comb (expr_to_raw e) seed.
 
@@ -70,7 +70,7 @@ Qed.
 
 Lemma freshness_translate_expr {ty} (e: Source.exp ty) (seed: ident):
   let '(ei, es, seed', pre_binders, pre_eqs, init_post, step_post) := translate_expr e seed in
-  freshness seed' pre_binders.
+  freshness seed' (pre_binders ++ map fst pre_eqs).
 Proof.
   destruct (translate_expr e seed) as [[[[[[]]]]]] eqn: translation.
   apply (Target.freshness_raw_to_comb translation).
@@ -78,7 +78,7 @@ Qed.
 
 Lemma isnext_translate_expr {ty} (e: Source.exp ty) (seed: ident):
   let '(ei, es, seed', pre_binders, pre_eqs, init_post, step_post) := translate_expr e seed in
-  forall x, In x (map fst pre_binders) -> exists n, x = iter n next_ident seed.
+  forall x, In x (map fst pre_binders ++ map (fun eq => fst (fst eq)) pre_eqs) -> exists n, x = iter n next_ident seed.
 Proof.
   destruct (translate_expr e seed) as [[[[[[]]]]]] eqn: translation.
   apply (Target.isnext_raw_to_comb translation).
@@ -86,7 +86,7 @@ Qed.
 
 Lemma nodup_translate_expr {ty} (e: Source.exp ty) (seed: ident):
   let '(ei, es, seed', pre_binders, pre_eqs, init_post, step_post) := translate_expr e seed in
-  NoDup (map fst pre_binders).
+  NoDup (map fst pre_binders ++ map (fun eq => fst (fst eq)) pre_eqs).
 Proof.
   destruct (translate_expr e seed) as [[[[[[]]]]]] eqn: translation.
   apply (Target.nodup_raw_to_comb translation).
@@ -94,7 +94,7 @@ Qed.
 
 Lemma translate_expr_assigned_init {ty} (e: Source.exp ty) (seed: ident):
   let '(ei, es, seed', pre_binders, pre_eqs, init_post, step_post) := translate_expr e seed in
-  Permutation (map Target.equation_dest (pre_eqs ++ init_post)) pre_binders.
+  Permutation (map Target.equation_dest init_post) pre_binders.
 Proof.
   destruct (translate_expr e seed) as [[[[[[]]]]]] eqn: translation.
   apply (Target.raw_to_comb_assigned_init translation).
@@ -102,10 +102,225 @@ Qed.
 
 Lemma translate_expr_assigned_step {ty} (e: Source.exp ty) (seed: ident):
   let '(ei, es, seed', pre_binders, pre_eqs, init_post, step_post) := translate_expr e seed in
-  Permutation (map Target.equation_dest (pre_eqs ++ step_post)) pre_binders.
+  Permutation (map Target.equation_dest step_post) pre_binders.
 Proof.
   destruct (translate_expr e seed) as [[[[[[]]]]]] eqn: translation.
   apply (Target.raw_to_comb_assigned_step translation).
+Qed.
+
+Lemma translate_expr_init_wd v {ty} {e: Source.exp ty} {n_in n_out n_locals} seed:
+  incl (Source.var_of_exp e) (n_in ++ n_out ++ n_locals) ->
+  let '(ei, es, seed', pre_binders, pre_eqs, init_post, step_post) := translate_expr e seed in
+  Forall (fun eq => incl (Target.var_of_exp (projT2 (snd eq))) (n_in ++ n_out ++ pre_binders ++ n_locals)) ((v, existT _ ty ei) :: init_post).
+Proof.
+  intros Hwd; revert seed; induction e as [ty c|[ty b]|ty1 ty op e IH|ty1 ty2 ty op e1 IH1 e2 IH2|ty e1 IH1 e2 IH2 e3 IH3];
+    intros seed; cbn; try (constructor; [|constructor]).
+  - intros ? [].
+  - exact Hwd.
+  - destruct op; cbn.
+    all: specialize (IH Hwd seed); unfold translate_expr in IH.
+    all: destruct (Target.raw_to_comb (expr_to_raw e) seed) as [[[[[[]]]]]].
+    3:{
+      constructor; [|constructor].
+      - intros ? [<-|[]]; apply in_or_app, or_intror, in_or_app, or_intror; left; exact eq_refl.
+      - refine (incl_trans _ _ _ (Forall_inv IH) _).
+        cbn.
+        apply incl_app_app; [apply incl_refl|].
+        apply incl_app_app; [apply incl_refl|].
+        intros ? h; right; exact h.
+      - refine (Forall_impl _ _ (Forall_inv_tail IH)).
+        clear; intros ? Hincl ? Hin.
+        specialize (Hincl _ Hin).
+        rewrite !in_app_iff in *; cbn; tauto.
+    }
+    all: constructor; [exact (Forall_inv IH)|exact (Forall_inv_tail IH)].
+  - cbn in Hwd; rewrite Source.var_of_exp_aux_eq in Hwd.
+    specialize (IH1 (fun _ h => Hwd _ (in_or_app _ _ _ (or_introl h))) seed).
+    specialize (IH2 (fun _ h => Hwd _ (in_or_app _ _ _ (or_intror h)))).
+    clear Hwd; unfold translate_expr in IH1, IH2.
+    destruct op; cbn.
+    all: destruct (Target.raw_to_comb (expr_to_raw e1) seed) as [[[[[[] seed2]]]]]; clear e1.
+    all: specialize (IH2 seed2).
+    all: destruct (Target.raw_to_comb (expr_to_raw e2) seed2) as [[[[[[] seed']]]]]; clear e2.
+    14:{
+      constructor; [|apply Forall_app; split].
+      - refine (incl_trans _ _ _ (Forall_inv IH1) _).
+        cbn.
+        apply incl_app_app; [apply incl_refl|].
+        apply incl_app_app; [apply incl_refl|].
+        apply incl_app_app; [|apply incl_refl].
+        intros ? h; apply in_or_app; left; exact h.
+      - refine (Forall_impl _ _ (Forall_inv_tail IH1)).
+        clear; intros ? Hincl ? Hin.
+        specialize (Hincl _ Hin).
+        cbn; rewrite !in_app_iff in *; tauto.
+      - refine (Forall_impl _ _ (Forall_inv_tail IH2)).
+        clear; intros ? Hincl ? Hin.
+        specialize (Hincl _ Hin).
+        cbn; rewrite !in_app_iff in *; tauto.
+    }
+    all: constructor; [|apply Forall_app; split; [refine (Forall_impl _ _ (Forall_inv_tail IH1))|refine (Forall_impl _ _ (Forall_inv_tail IH2))]].
+    2,3,5,6,8,9,11,12,14,15,17,18,20,21,23,24,26,27,29,30,32,33,35,36,38,39: clear; intros ? Hincl ? Hin.
+    2-27: specialize (Hincl _ Hin); cbn; rewrite !in_app_iff in *; tauto.
+    all: cbn; rewrite Target.var_of_exp_aux_eq.
+    all: apply incl_app; [refine (incl_trans _ _ _ (Forall_inv IH1) _)|refine (incl_trans _ _ _ (Forall_inv IH2) _)]; cbn.
+    all: apply incl_app_app; [apply incl_refl|].
+    all: apply incl_app_app; [apply incl_refl|].
+    all: apply incl_app_app; [|apply incl_refl].
+    all: intros ? h; apply in_or_app; tauto.
+  - cbn in Hwd; rewrite 2!Source.var_of_exp_aux_eq in Hwd.
+    specialize (IH1 (fun _ h => Hwd _ (in_or_app _ _ _ (or_introl h))) seed).
+    specialize (IH2 (fun _ h => Hwd _ (in_or_app _ _ _ (or_intror (in_or_app _ _ _ (or_introl h)))))).
+    specialize (IH3 (fun _ h => Hwd _ (in_or_app _ _ _ (or_intror (in_or_app _ _ _ (or_intror h)))))).
+    clear Hwd; unfold translate_expr in IH1, IH2, IH3.
+    destruct (Target.raw_to_comb (expr_to_raw e1) seed) as [[[[[[] seed2]]]]]; clear e1.
+    specialize (IH2 seed2).
+    destruct (Target.raw_to_comb (expr_to_raw e2) seed2) as [[[[[[] seed3]]]]]; clear e2.
+    specialize (IH3 seed3).
+    destruct (Target.raw_to_comb (expr_to_raw e3) seed3) as [[[[[[] seed']]]]]; clear e3.
+    constructor; [|apply Forall_app; split; [|apply Forall_app; split]].
+    2: refine (Forall_impl _ _ (Forall_inv_tail IH1)).
+    3: refine (Forall_impl _ _ (Forall_inv_tail IH2)).
+    4: refine (Forall_impl _ _ (Forall_inv_tail IH3)).
+    2-4: clear; intros ? Hincl ? Hin; specialize (Hincl _ Hin).
+    2-4: cbn; rewrite !in_app_iff in *; tauto.
+    cbn; rewrite 2!Target.var_of_exp_aux_eq.
+    repeat apply incl_app.
+    1: refine (incl_trans _ _ _ (Forall_inv IH1) _).
+    2: refine (incl_trans _ _ _ (Forall_inv IH2) _).
+    3: refine (incl_trans _ _ _ (Forall_inv IH3) _).
+    all: do 2 (apply incl_app_app; [apply incl_refl|]).
+    all: apply incl_app_app; [|apply incl_refl].
+    all: cbn; intros ? h; rewrite !in_app_iff; tauto.
+Qed.
+
+Lemma translate_expr_pre_wd {ty} {e: Source.exp ty} {n_in n_out n_locals} seed:
+  incl (Source.var_of_exp e) (n_in ++ n_out ++ n_locals) ->
+  let '(ei, es, seed', pre_binders, pre_eqs, init_post, step_post) := translate_expr e seed in
+  Forall (fun eq => In (snd eq, snd (fst eq)) (n_in ++ n_out ++ pre_binders ++ n_locals)) pre_eqs.
+Proof.
+  intros _; revert seed; induction e as [ty c|[ty b]|ty1 ty op e IH|ty1 ty2 ty op e1 IH1 e2 IH2|ty e1 IH1 e2 IH2 e3 IH3];
+    intros seed; cbn; try (constructor; [|constructor]).
+  - apply Forall_nil.
+  - apply Forall_nil.
+  - destruct op; cbn.
+    all: specialize (IH seed); unfold translate_expr in IH.
+    all: destruct (Target.raw_to_comb (expr_to_raw e) seed) as [[[[[[]]]]]].
+    3:{
+      constructor; [|refine (Forall_impl _ _ IH)].
+      2: clear; cbn; intros ? Hin; cbn; rewrite !in_app_iff in *; cbn; rewrite in_app_iff; tauto.
+      apply in_or_app, or_intror, in_or_app, or_intror; left; exact eq_refl.
+    }
+    all: exact IH.
+  - specialize (IH1 seed).
+    unfold translate_expr in IH1, IH2.
+    destruct op; cbn.
+    all: destruct (Target.raw_to_comb (expr_to_raw e1) seed) as [[[[[[] seed2]]]]]; clear e1.
+    all: specialize (IH2 seed2).
+    all: destruct (Target.raw_to_comb (expr_to_raw e2) seed2) as [[[[[[] seed']]]]]; clear e2.
+    all: apply Forall_app; split; [refine (Forall_impl _ _ IH1)|refine (Forall_impl _ _ IH2)].
+    all: clear; intros ? Hin.
+    all: rewrite !in_app_iff in *; tauto.
+  - unfold translate_expr in IH1, IH2, IH3.
+    specialize (IH1 seed).
+    destruct (Target.raw_to_comb (expr_to_raw e1) seed) as [[[[[[] seed2]]]]]; clear e1.
+    specialize (IH2 seed2).
+    destruct (Target.raw_to_comb (expr_to_raw e2) seed2) as [[[[[[] seed3]]]]]; clear e2.
+    specialize (IH3 seed3).
+    destruct (Target.raw_to_comb (expr_to_raw e3) seed3) as [[[[[[] seed']]]]]; clear e3.
+    apply Forall_app; split; [|apply Forall_app; split].
+    1: refine (Forall_impl _ _ IH1).
+    2: refine (Forall_impl _ _ IH2).
+    3: refine (Forall_impl _ _ IH3).
+    all: clear; intros ? Hin.
+    all: rewrite !in_app_iff in *; tauto.
+Qed.
+
+Lemma translate_expr_step_wd v {ty} {e: Source.exp ty} {n_in n_out n_locals} seed:
+  incl (Source.var_of_exp e) (n_in ++ n_out ++ n_locals) ->
+  let '(ei, es, seed', pre_binders, pre_eqs, init_post, step_post) := translate_expr e seed in
+  Forall (fun eq => incl (Target.var_of_exp (projT2 (snd eq))) ((n_in ++ n_out ++ pre_binders ++ n_locals) ++ map fst pre_eqs))
+    ((v, existT _ ty es) :: step_post).
+Proof.
+  intros Hwd; revert seed; induction e as [ty c|[ty b]|ty1 ty op e IH|ty1 ty2 ty op e1 IH1 e2 IH2|ty e1 IH1 e2 IH2 e3 IH3];
+    intros seed; cbn; try (constructor; [|constructor]).
+  - intros ? [].
+  - rewrite app_nil_r; exact Hwd.
+  - destruct op; cbn.
+    all: specialize (IH Hwd seed); unfold translate_expr in IH.
+    all: destruct (Target.raw_to_comb (expr_to_raw e) seed) as [[[[[[]]]]]].
+    3:{
+      constructor; [|constructor].
+      - intros ? [<-|[]]; apply in_or_app; right; left; exact eq_refl.
+      - refine (incl_trans _ _ _ (Forall_inv IH) _).
+        cbn.
+        apply incl_app_app; [|intros ? h; right; exact h].
+        do 2 (apply incl_app_app; [apply incl_refl|]).
+        intros ? h; right; exact h.
+      - refine (Forall_impl _ _ (Forall_inv_tail IH)).
+        clear; intros ? Hincl ? Hin.
+        specialize (Hincl _ Hin).
+        rewrite !in_app_iff in *; cbn; tauto.
+    }
+    all: constructor; [exact (Forall_inv IH)|exact (Forall_inv_tail IH)].
+  - cbn in Hwd; rewrite Source.var_of_exp_aux_eq in Hwd.
+    specialize (IH1 (fun _ h => Hwd _ (in_or_app _ _ _ (or_introl h))) seed).
+    specialize (IH2 (fun _ h => Hwd _ (in_or_app _ _ _ (or_intror h)))).
+    clear Hwd; unfold translate_expr in IH1, IH2.
+    destruct op; cbn.
+    all: destruct (Target.raw_to_comb (expr_to_raw e1) seed) as [[[[[[] seed2]]]]]; clear e1.
+    all: specialize (IH2 seed2).
+    all: destruct (Target.raw_to_comb (expr_to_raw e2) seed2) as [[[[[[] seed']]]]]; clear e2.
+    14:{
+      constructor; [|apply Forall_app; split].
+      - refine (incl_trans _ _ _ (Forall_inv IH2) _).
+        apply incl_app_app; [|intros ? h; rewrite map_app; apply in_or_app; right; exact h].
+        do 2 (apply incl_app_app; [apply incl_refl|]).
+        apply incl_app_app; [|apply incl_refl].
+        intros ? h; apply in_or_app; right; exact h.
+      - refine (Forall_impl _ _ (Forall_inv_tail IH1)).
+        clear; intros ? Hincl ? Hin.
+        specialize (Hincl _ Hin).
+        cbn; rewrite map_app, !in_app_iff in *; tauto.
+      - refine (Forall_impl _ _ (Forall_inv_tail IH2)).
+        clear; intros ? Hincl ? Hin.
+        specialize (Hincl _ Hin).
+        cbn; rewrite map_app, !in_app_iff in *; tauto.
+    }
+    all: constructor; [|apply Forall_app; split; [refine (Forall_impl _ _ (Forall_inv_tail IH1))|refine (Forall_impl _ _ (Forall_inv_tail IH2))]].
+    2,3,5,6,8,9,11,12,14,15,17,18,20,21,23,24,26,27,29,30,32,33,35,36,38,39: clear; intros ? Hincl ? Hin.
+    2-27: specialize (Hincl _ Hin); cbn; rewrite map_app, !in_app_iff in *; tauto.
+    all: cbn; rewrite Target.var_of_exp_aux_eq.
+    all: apply incl_app; [refine (incl_trans _ _ _ (Forall_inv IH1) _)|refine (incl_trans _ _ _ (Forall_inv IH2) _)]; cbn.
+    all: apply incl_app_app; [|intros ? h; rewrite map_app; apply in_or_app; tauto].
+    all: do 2 (apply incl_app_app; [apply incl_refl|]).
+    all: apply incl_app_app; [|apply incl_refl].
+    all: intros ? h; apply in_or_app; tauto.
+  - cbn in Hwd; rewrite 2!Source.var_of_exp_aux_eq in Hwd.
+    specialize (IH1 (fun _ h => Hwd _ (in_or_app _ _ _ (or_introl h))) seed).
+    specialize (IH2 (fun _ h => Hwd _ (in_or_app _ _ _ (or_intror (in_or_app _ _ _ (or_introl h)))))).
+    specialize (IH3 (fun _ h => Hwd _ (in_or_app _ _ _ (or_intror (in_or_app _ _ _ (or_intror h)))))).
+    clear Hwd; unfold translate_expr in IH1, IH2, IH3.
+    destruct (Target.raw_to_comb (expr_to_raw e1) seed) as [[[[[[] seed2]]]]]; clear e1.
+    specialize (IH2 seed2).
+    destruct (Target.raw_to_comb (expr_to_raw e2) seed2) as [[[[[[] seed3]]]]]; clear e2.
+    specialize (IH3 seed3).
+    destruct (Target.raw_to_comb (expr_to_raw e3) seed3) as [[[[[[] seed']]]]]; clear e3.
+    constructor; [|apply Forall_app; split; [|apply Forall_app; split]].
+    2: refine (Forall_impl _ _ (Forall_inv_tail IH1)).
+    3: refine (Forall_impl _ _ (Forall_inv_tail IH2)).
+    4: refine (Forall_impl _ _ (Forall_inv_tail IH3)).
+    2-4: clear; intros ? Hincl ? Hin; specialize (Hincl _ Hin).
+    2-4: cbn; rewrite !map_app, !in_app_iff in *; tauto.
+    cbn; rewrite 2!Target.var_of_exp_aux_eq.
+    repeat apply incl_app.
+    1: refine (incl_trans _ _ _ (Forall_inv IH1) _).
+    2: refine (incl_trans _ _ _ (Forall_inv IH2) _).
+    3: refine (incl_trans _ _ _ (Forall_inv IH3) _).
+    all: apply incl_app_app; [|intros ? h; rewrite !map_app, !in_app_iff; tauto].
+    all: do 2 (apply incl_app_app; [apply incl_refl|]).
+    all: apply incl_app_app; [|apply incl_refl].
+    all: cbn; intros ? h; rewrite !in_app_iff; tauto.
 Qed.
 
 Fixpoint translate_equations (eqs: list Source.equation) (seed: ident): (
@@ -113,7 +328,7 @@ Fixpoint translate_equations (eqs: list Source.equation) (seed: ident): (
     * list Target.equation (* step *)
     * ident (* New identifier origin *)
     * list binder (* Variables created for pre *)
-    * list Target.equation (* pre equations *)
+    * list (binder * ident)(* pre equations *)
     (* Equations to merge with the regular equations *)
     (* for init: 
       prex = undef (a variable initialised later)
@@ -167,7 +382,7 @@ Qed.
 
 Lemma freshness_translate_equations (eqs: list Source.equation) (seed: ident):
   let '(init_eqs, step_eqs, seed', pre_binders, pre_eqs, init_post, step_post) := translate_equations eqs seed in
-  freshness seed' pre_binders.
+  freshness seed' (pre_binders ++ map fst pre_eqs).
 Proof.
   destruct (translate_equations eqs seed) as [[[[[[init_eqs step_eqs] seed'] pre_binders] pre_eqs] init_post] step_post] eqn: translation.
   induction eqs as [| eq eqs IH] in seed, seed', pre_binders, init_eqs, step_eqs, pre_eqs, init_post, step_post, translation |- *.
@@ -183,12 +398,13 @@ Proof.
     injection translation as <- <- <- <- <- <- <-.
     specialize (IH _ _ _ _ _ _ _ _ unfoldtrans).
     apply (freshness_later_e nextseed_expr) in IH.
-    apply (freshness_fusion freshness_expr IH).
+    refine (freshness_permutation (freshness_fusion freshness_expr IH) _).
+    rewrite map_app, !app_assoc; apply Permutation_app_tail; rewrite <-!app_assoc; apply Permutation_app_head, Permutation_app_comm.
 Qed.
 
 Lemma isnext_translate_equations (eqs: list Source.equation) (seed: ident):
   let '(init_eqs, step_eqs, seed', pre_binders, pre_eqs, init_post, step_post) := translate_equations eqs seed in
-  forall x, In x (map fst pre_binders) -> exists n, x = iter n next_ident seed.
+  forall x, In x (map fst pre_binders ++ map (fun eq => fst (fst eq)) pre_eqs) -> exists n, x = iter n next_ident seed.
 Proof.
   destruct (translate_equations eqs seed) as [[[[[[init_eqs step_eqs] seed'] pre_binders] pre_eqs] init_post] step_post] eqn: translation.
   induction eqs as [| eq eqs IH] in seed, seed', pre_binders, init_eqs, step_eqs, pre_eqs, init_post, step_post, translation |- *.
@@ -208,20 +424,22 @@ Proof.
     destruct nextseed as [nseed nextseed].
     rewrite nextseed in isnext_expr.
     specialize (isnext_expr x).
-    rewrite map_app in isin.
-    apply in_app_or in isin.
-    destruct isin as [isin | isin].
-    2: tauto.
-    specialize (isnext_expr isin).
-    destruct isnext_expr as [n isnext_expr].
-    rewrite <- Nat.iter_add in isnext_expr.
-    exists (n + nseed).
-    assumption.
+    cbn in IH, isnext_expr, isin.
+    rewrite !map_app in isin.
+    rewrite in_app_iff in IH, isnext_expr, isin; rewrite !in_app_iff in isin.
+    destruct isin as [[isin | isin] | [isin | isin]].
+    2,4: tauto.
+    1: specialize (isnext_expr (or_introl isin)).
+    2: specialize (isnext_expr (or_intror isin)).
+    all: destruct isnext_expr as [n isnext_expr].
+    all: rewrite <- Nat.iter_add in isnext_expr.
+    all: exists (n + nseed).
+    all: assumption.
 Qed.
 
 Lemma nodup_translate_equations (eqs: list Source.equation) (seed: ident):
   let '(init_eqs, step_eqs, seed', pre_binders, pre_eqs, init_post, step_post) := translate_equations eqs seed in
-  NoDup (map fst pre_binders).
+  NoDup (map fst pre_binders ++ map (fun eq => fst (fst eq)) pre_eqs).
 Proof.
   destruct (translate_equations eqs seed) as [[[[[[init_eqs step_eqs] seed'] pre_binders] pre_eqs] init_post] step_post] eqn: translation.
   induction eqs as [| eq eqs IH] in seed, seed', pre_binders, init_eqs, step_eqs, pre_eqs, init_post, step_post, translation |- *.
@@ -236,21 +454,20 @@ Proof.
     destruct (translate_expr expr seed0) as [[[[[[ei2 es2] seed2] binders2] pre_eqs2] init_post2] step_post2].
     injection translation as <- <- <- <- <- <- <-.
     specialize (IH _ _ _ _ _ _ _ _ unfoldtrans).
-    rewrite map_app.
-    apply NoDup_app.
-    1, 2: assumption.
-    intros x isin2.
-    intro isin0.
-    specialize (isnext  x isin2).
+    cbn in *; rewrite !map_app.
+    refine (Permutation_NoDup _ (NoDup_app nodup_expr IH _)).
+    1: rewrite !app_assoc; apply Permutation_app_tail; rewrite <-!app_assoc; apply Permutation_app_head, Permutation_app_comm.
+    intros x isin2 isin0.
+    specialize (isnext x isin2).
     destruct isnext as [n isnext].
     specialize (freshness_trans n).
-    rewrite isnext in isin0.
+    rewrite isnext, <-(map_map fst fst), <-map_app in isin0.
     contradiction.
 Qed.
 
 Lemma translate_equations_assigned_init (eqs: list Source.equation) (seed: ident):
   let '(init_eqs, step_eqs, seed', pre_binders, pre_eqs, init_post, step_post) := translate_equations eqs seed in
-  Permutation (map Target.equation_dest (pre_eqs ++ init_post)) pre_binders.
+  Permutation (map Target.equation_dest init_post) pre_binders.
 Proof.
   destruct (translate_equations eqs seed) as [[[[[[init_eqs step_eqs] seed'] pre_binders] pre_eqs] init_post] step_post] eqn: translation.
   induction eqs as [| eq eqs IH] in seed, seed', pre_binders, init_eqs, step_eqs, pre_eqs, init_post, step_post, translation |- *.
@@ -263,22 +480,12 @@ Proof.
     destruct (translate_expr expr seed0) as [[[[[[ei2 es2] seed2] binders2] pre_eqs2] init_post2] step_post2].
     injection translation as <- <- <- <- <- <- <-.
     specialize (IH _ _ _ _ _ _ _ _ unfoldtrans).
-    rewrite !map_app.
-    rewrite map_app in IH.
-    rewrite map_app in perm_expr.
-    rewrite (Permutation_app_comm (map Target.equation_dest pre_eqs2)).
-    rewrite <- app_assoc.
-    rewrite Permutation_app_comm.
-    rewrite <- !app_assoc.
-    rewrite app_assoc.
-    rewrite (Permutation_app_comm (map Target.equation_dest init_post0)).
-    apply Permutation_app.
-    all: assumption.
+    rewrite !map_app, IH, perm_expr; apply Permutation_refl.
 Qed.
 
 Lemma translate_equations_assigned_step (eqs: list Source.equation) (seed: ident):
   let '(init_eqs, step_eqs, seed', pre_binders, pre_eqs, init_post, step_post) := translate_equations eqs seed in
-  Permutation (map Target.equation_dest (pre_eqs ++ step_post)) pre_binders.
+  Permutation (map Target.equation_dest step_post) pre_binders.
 Proof.
   destruct (translate_equations eqs seed) as [[[[[[init_eqs step_eqs] seed'] pre_binders] pre_eqs] init_post] step_post] eqn: translation.
   induction eqs as [| eq eqs IH] in seed, seed', pre_binders, init_eqs, step_eqs, pre_eqs, init_post, step_post, translation |- *.
@@ -291,17 +498,7 @@ Proof.
     destruct (translate_expr expr seed0) as [[[[[[ei2 es2] seed2] binders2] pre_eqs2] init_post2] step_post2].
     injection translation as <- <- <- <- <- <- <-.
     specialize (IH _ _ _ _ _ _ _ _ unfoldtrans).
-    rewrite !map_app.
-    rewrite map_app in IH.
-    rewrite map_app in perm_expr.
-    rewrite (Permutation_app_comm (map Target.equation_dest pre_eqs2)).
-    rewrite <- app_assoc.
-    rewrite Permutation_app_comm.
-    rewrite <- !app_assoc.
-    rewrite app_assoc.
-    rewrite (Permutation_app_comm (map Target.equation_dest step_post0)).
-    apply Permutation_app.
-    all: assumption.
+    rewrite !map_app, IH, perm_expr; apply Permutation_refl.
 Qed.
 
 Lemma translate_equations_conservation_init (eqs: list Source.equation) (seed: ident):
@@ -347,7 +544,7 @@ Qed.
 Lemma translate_init_assigned {n_body n_out n_locals} (n_seed: ident)
   (n_vars_all_assigned : Permutation (map Source.equation_dest n_body) (n_out ++ n_locals)) :
   let '(init_eqs, step_eqs, new_seed, pre_binders, pre_eqs, init_post_eqs, step_post_eqs) := translate_equations n_body n_seed in
-  Permutation (map Target.equation_dest pre_eqs ++ map Target.equation_dest (init_eqs ++ init_post_eqs)) (n_out ++ pre_binders ++ n_locals).
+  Permutation (map Target.equation_dest (init_eqs ++ init_post_eqs)) (n_out ++ pre_binders ++ n_locals).
 Proof.
   assert (conservation_init := translate_equations_conservation_init n_body n_seed).
   assert (assigned_init := translate_equations_assigned_init n_body n_seed).
@@ -359,17 +556,15 @@ Proof.
   rewrite (Permutation_app_comm n_out).
   rewrite <- !app_assoc.
   rewrite <- n_vars_all_assigned.
-  rewrite !app_assoc.
   apply Permutation_app.
   2: apply Permutation_refl.
-  rewrite <- map_app.
   assumption.
 Qed.
 
 Lemma translate_step_assigned {n_body n_out n_locals} (n_seed: ident)
   (n_vars_all_assigned : Permutation (map Source.equation_dest n_body) (n_out ++ n_locals)) :
   let '(init_eqs, step_eqs, new_seed, pre_binders, pre_eqs, init_post_eqs, step_post_eqs) := translate_equations n_body n_seed in
-  Permutation (map Target.equation_dest pre_eqs ++ map Target.equation_dest (step_eqs ++ step_post_eqs)) (n_out ++ pre_binders ++ n_locals).
+  Permutation (map Target.equation_dest (step_eqs ++ step_post_eqs)) (n_out ++ pre_binders ++ n_locals).
 Proof.
   assert (conservation_step := translate_equations_conservation_step n_body n_seed).
   assert (assigned_step := translate_equations_assigned_step n_body n_seed).
@@ -381,10 +576,8 @@ Proof.
   rewrite (Permutation_app_comm n_out).
   rewrite <- !app_assoc.
   rewrite <- n_vars_all_assigned.
-  rewrite !app_assoc.
   apply Permutation_app.
   2: apply Permutation_refl.
-  rewrite <- map_app.
   assumption.
 Qed.
 
@@ -392,11 +585,12 @@ Lemma translate_vars_unique {n_in n_out n_locals n_seed} (n_body: list Source.eq
   (n_vars_unique : NoDup (map fst (n_in ++ n_out ++ n_locals)))
   (n_seed_always_fresh : freshness n_seed (n_in ++ n_out ++ n_locals)) :
   let '(init_eqs, step_eqs, new_seed, pre_binders, pre_eqs, init_post_eqs, step_post_eqs) := translate_equations n_body n_seed in
-  NoDup (map fst (n_in ++ n_out ++ pre_binders ++ n_locals)).
+  NoDup (map fst (n_in ++ n_out ++ pre_binders ++ n_locals) ++ map (fun eq => fst (fst eq)) pre_eqs).
 Proof.
   assert (nodup_translate := nodup_translate_equations n_body n_seed).
   assert (isnext := isnext_translate_equations n_body n_seed).
   destruct (translate_equations n_body n_seed) as [[[[[[init_eqs step_eqs] seed'] pre_binders] pre_eqs] init_post] step_post].
+  rewrite <-(map_map fst fst), <-map_app.
   rewrite !map_app.
   rewrite !map_app in n_vars_unique.
   unfold freshness in n_seed_always_fresh.
@@ -406,10 +600,10 @@ Proof.
   rewrite (Permutation_app_comm (map fst pre_binders)).
   rewrite <- app_assoc.
   rewrite Permutation_app_comm.
-  rewrite <- !app_assoc.
+  rewrite 2!app_assoc, <-app_assoc, <-(app_assoc (map _ _)), map_map.
   apply NoDup_app.
   1, 2: assumption.
-  intros x isin.
+  intros x f isin; revert f.
   specialize (isnext x isin).
   destruct isnext as [n isnext].
   rewrite isnext.
@@ -419,7 +613,7 @@ Qed.
 Lemma translate_seed_always_fresh {n_in n_out n_locals n_seed} (n_body: list Source.equation)
   (n_seed_always_fresh : freshness n_seed (n_in ++ n_out ++ n_locals)) :
   let '(init_eqs, step_eqs, new_seed, pre_binders, pre_eqs, init_post_eqs, step_post_eqs) := translate_equations n_body n_seed in
-  freshness new_seed (n_in ++ n_out ++ pre_binders ++ n_locals).
+  freshness new_seed ((n_in ++ n_out ++ pre_binders ++ n_locals) ++ map fst pre_eqs).
 Proof.
   assert (fresh_translate := freshness_translate_equations n_body n_seed).
   assert (nextseed := translate_equations_nextseed n_body n_seed).
@@ -429,11 +623,10 @@ Proof.
   unfold freshness in n_seed_always_fresh.
   rewrite !map_app in n_seed_always_fresh.
   rewrite app_assoc in isin.
+  rewrite (Permutation_app_comm (map _ pre_binders)) in isin.
+  rewrite app_assoc, <-app_assoc, <-(map_app _ pre_binders) in isin.
   rewrite Permutation_app_comm in isin.
-  rewrite (Permutation_app_comm (map fst pre_binders)) in isin.
-  rewrite <- app_assoc in isin.
-  rewrite Permutation_app_comm in isin.
-  rewrite <- !app_assoc in isin.
+  rewrite <-app_assoc in isin.
   apply in_app_or in isin.
   destruct nextseed as [nseed nextseed].
   specialize (fresh_translate n).
@@ -478,6 +671,75 @@ Proof.
     all: constructor 2; assumption.
 Qed.
 
+Lemma translate_init_wd {n_in n_out n_locals n_body} n_seed:
+  Forall (fun eq => incl (Source.var_of_exp (projT2 (snd eq))) (n_in ++ n_out ++ n_locals)) n_body ->
+  let '(init_eqs, step_eqs, new_seed, pre_binders, pre_eqs, init_post_eqs, step_post_eqs) := translate_equations n_body n_seed in
+  Forall (fun eq => incl (Target.var_of_exp (projT2 (snd eq))) (n_in ++ n_out ++ pre_binders ++ n_locals)) (init_eqs ++ init_post_eqs).
+Proof.
+  intros n_all_vars_exist.
+  induction n_body as [|[eqid [eqty eqeq]] n_body IH].
+  1: apply Forall_nil.
+  simpl.
+  specialize (IH (Forall_inv_tail n_all_vars_exist)).
+  destruct (translate_equations n_body n_seed) as [[[[[[init_eqs step_eqs] seed1] pre_binders] pre_eqs] init_post] step_post].
+  assert (Hexpr := translate_expr_init_wd eqid seed1 (Forall_inv n_all_vars_exist)); cbn in Hexpr; unfold translate_expr.
+  clear - IH Hexpr.
+  destruct (Target.raw_to_comb (expr_to_raw eqeq) seed1) as [[[[[[]]]]]]; cbn in *.
+  apply Forall_app in IH.
+  apply Forall_cons; [refine (incl_trans _ _ _ (Forall_inv Hexpr) _)|apply Forall_app; split; [|apply Forall_app; split]].
+  2: refine (Forall_impl _ _ (proj1 IH)).
+  3: refine (Forall_impl _ _ (Forall_inv_tail Hexpr)).
+  4: refine (Forall_impl _ _ (proj2 IH)).
+  1: clear; intros ? Hincl.
+  2-4: clear; intros ? Hincl ? Hin; specialize (Hincl _ Hin); clear - Hincl.
+  all: rewrite !in_app_iff in *; tauto.
+Qed.
+
+Lemma translate_pre_wd {n_in n_out n_locals n_body} n_seed:
+  Forall (fun eq => incl (Source.var_of_exp (projT2 (snd eq))) (n_in ++ n_out ++ n_locals)) n_body ->
+  let '(init_eqs, step_eqs, new_seed, pre_binders, pre_eqs, init_post_eqs, step_post_eqs) := translate_equations n_body n_seed in
+  Forall (fun eq => In (snd eq, snd (fst eq)) (n_in ++ n_out ++ pre_binders ++ n_locals)) pre_eqs.
+Proof.
+  intros n_all_vars_exist.
+  induction n_body as [|[eqid [eqty eqeq]] n_body IH].
+  1: apply Forall_nil.
+  simpl.
+  specialize (IH (Forall_inv_tail n_all_vars_exist)).
+  destruct (translate_equations n_body n_seed) as [[[[[[init_eqs step_eqs] seed1] pre_binders] pre_eqs] init_post] step_post].
+  assert (Hexpr := translate_expr_pre_wd seed1 (Forall_inv n_all_vars_exist)); cbn in Hexpr; unfold translate_expr.
+  clear - IH Hexpr.
+  destruct (Target.raw_to_comb (expr_to_raw eqeq) seed1) as [[[[[[]]]]]]; cbn in *.
+  apply Forall_app; split.
+  1: refine (Forall_impl _ _ Hexpr).
+  2: refine (Forall_impl _ _ IH).
+  all: clear; intros ? Hin; clear - Hin.
+  all: rewrite !in_app_iff in *; tauto.
+Qed.
+
+Lemma translate_step_wd {n_in n_out n_locals n_body} n_seed:
+  Forall (fun eq => incl (Source.var_of_exp (projT2 (snd eq))) (n_in ++ n_out ++ n_locals)) n_body ->
+  let '(init_eqs, step_eqs, new_seed, pre_binders, pre_eqs, init_post_eqs, step_post_eqs) := translate_equations n_body n_seed in
+  Forall (fun eq => incl (Target.var_of_exp (projT2 (snd eq))) ((n_in ++ n_out ++ pre_binders ++ n_locals) ++ map fst pre_eqs)) (step_eqs ++ step_post_eqs).
+Proof.
+  intros n_all_vars_exist.
+  induction n_body as [|[eqid [eqty eqeq]] n_body IH].
+  1: apply Forall_nil.
+  simpl.
+  specialize (IH (Forall_inv_tail n_all_vars_exist)).
+  destruct (translate_equations n_body n_seed) as [[[[[[init_eqs step_eqs] seed1] pre_binders] pre_eqs] init_post] step_post].
+  assert (Hexpr := translate_expr_step_wd eqid seed1 (Forall_inv n_all_vars_exist)); cbn in Hexpr; unfold translate_expr.
+  clear - IH Hexpr.
+  destruct (Target.raw_to_comb (expr_to_raw eqeq) seed1) as [[[[[[]]]]]]; cbn in *.
+  apply Forall_app in IH.
+  apply Forall_cons; [refine (incl_trans _ _ _ (Forall_inv Hexpr) _)|apply Forall_app; split; [|apply Forall_app; split]].
+  2: refine (Forall_impl _ _ (proj1 IH)).
+  3: refine (Forall_impl _ _ (Forall_inv_tail Hexpr)).
+  4: refine (Forall_impl _ _ (proj2 IH)).
+  1: clear; intros ? Hincl.
+  2-4: clear; intros ? Hincl ? Hin; specialize (Hincl _ Hin); clear - Hincl.
+  all: rewrite ?map_app, !in_app_iff in *; tauto.
+Qed.
+
 
 Definition translate_node (node: Source.node) : Result.t type Target.node.
 Proof.
@@ -506,6 +768,9 @@ Proof.
   assert (step_assigned := translate_step_assigned n_seed n_vars_all_assigned).
   assert (vars_unique := translate_vars_unique n_body n_vars_unique n_seed_always_fresh).
   assert (fresh_seed := translate_seed_always_fresh n_body n_seed_always_fresh).
+  assert (init_wd := translate_init_wd n_seed n_all_vars_exist).
+  assert (pre_wd := translate_pre_wd n_seed n_all_vars_exist).
+  assert (step_wd := translate_step_wd n_seed n_all_vars_exist).
 
   destruct (translate_equations n_body n_seed) as [
     [[[[[init_eqs
@@ -546,6 +811,9 @@ Proof.
   remember (translate_step_assigned n0_seed n0_vars_all_assigned) as step_assigned eqn: tmp; clear tmp.
   remember (translate_vars_unique n0_body n0_vars_unique n0_seed_always_fresh) as vars_unique eqn: tmp; clear tmp.
   remember (translate_seed_always_fresh n0_body n0_seed_always_fresh) as seed_fresh eqn: tmp; clear tmp.
+  remember (translate_init_wd n0_seed n0_all_vars_exist) as init_wd eqn: tmp; clear tmp.
+  remember (translate_pre_wd n0_seed n0_all_vars_exist) as pre_wd eqn: tmp; clear tmp.
+  remember (translate_step_wd n0_seed n0_all_vars_exist) as step_wd eqn: tmp; clear tmp.
   destruct (translate_equations n0_body n0_seed) as [[[[[[trans_init trans_step] trans_seed] trans_pre_binders] trans_pre_eqs] trans_init_eqs] trans_step_eqs] eqn: translation.
   subst.
   unfold Source.sem_node, Target.sem_node, Target.n_vars, Target.n_init, Target.n_in, Target.n_out, Target.n_locals, Target.n_step, Target.n_pre, Source.n_body.
@@ -553,7 +821,7 @@ Proof.
   intro sem_target.
   intros idn ty expr s inbody ismapped time.
 
-  specialize (sem_target idn ty).
+  specialize (sem_target idn ty) as [sem_target sem_target_pre].
   assert (id_is_var : In (idn, ty) (n0_in ++ n0_out ++ trans_pre_binders ++ n0_locals)).
   {
    assert (id_is_var2 : In (idn, ty) (n0_out ++ n0_locals)).
